@prefix : <http://bim.aalto.fi/DiCtion/Ontology/> .
@prefix owl: <http://www.w3.org/2002/07/owl#> .
@prefix rdf: <http://www.w3.org/1999/02/22-rdf-syntax-ns#> .
@prefix xml: <http://www.w3.org/XML/1998/namespace> .
@prefix xsd: <http://www.w3.org/2001/XMLSchema#> .
@prefix rdfs: <http://www.w3.org/2000/01/rdf-schema#> .
@base <http://bim.aalto.fi/DiCtion/Ontology/> .

<http://bim.aalto.fi/DiCtion/Ontology/> rdf:type owl:Ontology ;
                                         owl:versionIRI <http://bim.aalto.fi/DiCtion/Ontology/ConstructionOrganization/0.9.1> ;
                                         rdfs:comment "Seppo Torma"@en ,
                                                      "This Construction Organization ontology is known as one module of SSP ontology of DiCtion project. The purpose of this module is to support data sharing of the organization and business information that related to the construction project. This module can be used in organization-related information management use cases."@en ,
                                                      "Yuan Zheng"@en ;
                                         owl:versionInfo "0.9.1" .

#################################################################
#    Annotation properties
#################################################################

###  http://purl.org/dc/terms/creator
<http://purl.org/dc/terms/creator> rdf:type owl:AnnotationProperty .


#################################################################
#    Object Properties
#################################################################

###  http://bim.aalto.fi/DiCtion/Ontology/belongsTo
:belongsTo rdf:type owl:ObjectProperty ;
           rdfs:domain :Person ;
           rdfs:range :Organization ;
           rdfs:comment "Relation of Personnel affiliation between a Person and a Organization."@en .


###  http://bim.aalto.fi/DiCtion/Ontology/depandsOn
:depandsOn rdf:type owl:ObjectProperty ;
           rdfs:domain :Obligation ;
           rdfs:range :DependencyConstraint ;
           rdfs:comment "Relation between an Obligation and its correspondent dependency constraints"@en .


###  http://bim.aalto.fi/DiCtion/Ontology/fulfilObligation
:fulfilObligation rdf:type owl:ObjectProperty ;
                  rdfs:domain :Actor ;
                  rdfs:range :Obligation ;
                  rdfs:comment "A relation between an actor who should fulfil obligation and the obligation"@en .


###  http://bim.aalto.fi/DiCtion/Ontology/hasObject
:hasObject rdf:type owl:ObjectProperty ;
           rdfs:domain :Delivery ;
           rdfs:range :DomainObject ;
           rdfs:comment "A relation of between object-relevant concepts and their related domain object"@en .


###  http://bim.aalto.fi/DiCtion/Ontology/isPromiseeof
:isPromiseeof rdf:type owl:ObjectProperty ;
              rdfs:domain :Actor ;
              rdfs:range :Contract ;
              rdfs:comment "Relation that indicates an actor is the promisee of correspondent contract"@en .


###  http://bim.aalto.fi/DiCtion/Ontology/isPromisorof
:isPromisorof rdf:type owl:ObjectProperty ;
              rdfs:domain :Actor ;
              rdfs:range :Contract ;
              rdfs:comment "Relation that indicates an actor is the promisor of correspondent contract"@en .


###  http://bim.aalto.fi/DiCtion/Ontology/isResponsiblefor
:isResponsiblefor rdf:type owl:ObjectProperty ;
                  rdfs:domain :Actor ;
                  rdfs:range :Activity ;
                  rdfs:comment "relation between an actor and its responsible activity"@en .


###  http://bim.aalto.fi/DiCtion/Ontology/receiveObligation
:receiveObligation rdf:type owl:ObjectProperty ;
                   rdfs:domain :Actor ;
                   rdfs:range :Obligation ;
                   rdfs:comment "A relation between an actor who receive obligation and the obligation"@en .


###  http://bim.aalto.fi/DiCtion/Ontology/retricts
:retricts rdf:type owl:ObjectProperty ;
          rdfs:domain :Contract ;
          rdfs:range :Obligation ;
          rdfs:comment "Relation between Contract and Obligation that indicates obligation is restricted by corresdented statement in Contract" .


#################################################################
#    Classes
#################################################################

###  http://bim.aalto.fi/DiCtion/Ontology/Activity
:Activity rdf:type owl:Class ;
          rdfs:subClassOf :DomainObject ;
          rdfs:comment "Activity is the concept refers to all the works (or aggregations of works) that carried out in a construction project."@en .


###  http://bim.aalto.fi/DiCtion/Ontology/Actor
:Actor rdf:type owl:Class ;
       rdfs:subClassOf :Resource ;
       rdfs:comment "Actor is a subclass of Resource, which refers to all the agents that are responsible of activities."@en .


###  http://bim.aalto.fi/DiCtion/Ontology/Company
:Company rdf:type owl:Class ;
         rdfs:subClassOf :Organization ;
         rdfs:comment "A commercial business unit that involves in the process."@en .


###  http://bim.aalto.fi/DiCtion/Ontology/Contract
:Contract rdf:type owl:Class ;
          rdfs:comment "An agreement that declares the obligations and duties for each of the participants."@en .


###  http://bim.aalto.fi/DiCtion/Ontology/Delivery
:Delivery rdf:type owl:Class ;
          rdfs:subClassOf :Obligation ;
          rdfs:comment "the action of delivering required objects"@en .


###  http://bim.aalto.fi/DiCtion/Ontology/DependencyConstraint
:DependencyConstraint rdf:type owl:Class ;
                      rdfs:comment "Constraints to formalize the obligations"@en .


###  http://bim.aalto.fi/DiCtion/Ontology/DomainObject
:DomainObject rdf:type owl:Class ;
              rdfs:comment "Domain objects is a abstract concept that refers to all the central objects that are discussed in the construction project planning and management. Sub-classes of the domain object include the 'Activity','Group','Information Entity','Physical Entity',and 'Resource'. Domain objects can have their specific classification that is defined by certain classification scheme in the construction domain, such as Uniformat, Omniclass and etc. Meanwhile, they can also have their level assignment that is defined based level of detail, level of development, level of application and etc."@en .


###  http://bim.aalto.fi/DiCtion/Ontology/DueDate
:DueDate rdf:type owl:Class ;
         rdfs:subClassOf :DependencyConstraint ;
         rdfs:comment "An time constraint of the final time of fulfiling the obligation"@en .


###  http://bim.aalto.fi/DiCtion/Ontology/LeadTime
:LeadTime rdf:type owl:Class ;
          rdfs:subClassOf :DependencyConstraint ;
          rdfs:comment "An time constraint of the time between the initiation and completion of a production process."@en .


###  http://bim.aalto.fi/DiCtion/Ontology/Obligation
:Obligation rdf:type owl:Class ;
            rdfs:comment "Obligation refers to specific duty of an actor to act, which is determined base on the contract."@en .


###  http://bim.aalto.fi/DiCtion/Ontology/Organization
:Organization rdf:type owl:Class ;
              rdfs:subClassOf :Actor ;
              rdfs:comment "An organized group of people with a particular purpose involves in the process."@en .


###  http://bim.aalto.fi/DiCtion/Ontology/Payment
:Payment rdf:type owl:Class ;
         rdfs:subClassOf :Obligation ;
         rdfs:comment "the action or process of paying"@en .


###  http://bim.aalto.fi/DiCtion/Ontology/Person
:Person rdf:type owl:Class ;
        rdfs:subClassOf :Actor ;
        rdfs:comment "A human being involves in the process."@en .


###  http://bim.aalto.fi/DiCtion/Ontology/Resource
:Resource rdf:type owl:Class ;
          rdfs:subClassOf :DomainObject ;
          rdfs:comment "Resource concept refers to the objects within a construction project that participate in value-adding transformations but that are not ultimately transformed themselves (such as labors and equipments)."@en .


###  Generated by the OWL API (version 5.1.7) https://github.com/owlcs/owlapi/
